minor updates

model/agp32RelationScript.sml
@@ -284,6 +284,8 @@ Definition Inv_Rel_def:
    (enable_stg 2 si ==> enable_stg 3 s ==> ~isJump_hw_op s ==> ~reg_data_hazard s ==> I (3,SUC t) = NONE ==>
     isJump_hw_op si) /\
    (~enable_stg 2 si ==> ~isJump_hw_op s ==> I (2,t) = NONE ==> s.ID.ID_opc = 15w) /\
+   (isJump_hw_op s ==> I (1,t) = NONE) /\
+   (isJump_hw_op s ==> I (2,t) = NONE) /\
    (I (3,t) = NONE ==> (s.EX.EX_opc = 16w \/ s.EX.EX_opc = 15w)) /\
    (I (3,t) = NONE ==> ~s.EX.EX_write_reg) /\
    (I (4,t) = NONE ==> (s.MEM.MEM_opc = 16w \/ s.MEM.MEM_opc = 15w)) /\
